Semantics.v
@@ -124,53 +124,6 @@ Inductive write_state (m:state) (l:loc) (π:accesses) (w:val) (m':state) : Prop 
       m' = m[l := v2] ->
       write_state m l π w m'.
 
-(* ---------------------------------------------------------------------- *)
-(** Semantics of the low-level memory accesses *)
-
-(** m(l)[o] = v *)
-
-(* TODO: Move to LibList? *)
-Definition list_slice {A:Type} (l:list A) (i:int) (n:int) (lr:list A) : Prop :=
-      lr = take n (drop i l)
-  /\  0 <= n
-  /\  0 <= i
-  /\  i + n <= length l.
-
-Inductive read_ll_state (m:state) (l:loc) (o:offset) (n:size) (ws':words) : Prop :=
-  | read_ll_state_intro : forall ws,
-      l \indom m ->
-      m[l] = val_words ws ->
-      list_slice ws o n ws' ->
-      read_ll_state m l o n ws'.
-
-(** m[l := m(l)[π := w]] = m' *)
-
-(* TODO: Move to LibList? *)
-Definition list_slice_update {A:Type} (l:list A) (i:int) (l':list A) (lr:list A) : Prop :=
-      lr = (take i l) ++ l' ++ (drop (i + length l') l)
-  /\  0 <= i
-  /\  i + length l' <= length l.
-
-Inductive write_ll_state (m:state) (l:loc) (o:offset) (ws':words) (m':state) : Prop :=
-  | write_ll_state_intro : forall ws ws'',
-      l \indom m ->
-      m[l] = val_words ws ->
-      list_slice_update ws o ws' ws'' ->
-      m' = m[l := (val_words ws'')] ->
-      write_ll_state m l o ws' m'.
-
-(*
-Inductive write_ll_state (m:state) (p:loc) (ws':words) (m':state) : Prop :=
-  | write_ll_state_intro : forall l o ws ws'',
-      l \indom m ->
-      index m[l] o ->
-      p = l + o ->
-      m[l] = val_words ws ->
-      list_slice_update ws o ws' ws'' ->
-      m' = m[l := (val_words ws'')] ->
-      write_ll_state m p ws' m'.
-*)
-
 
 (* ---------------------------------------------------------------------- *)
 (** Big-step evaluation *)
