TrSoA.v
@@ -1,0 +1,228 @@
+(**
+
+This file describes transformations of the layout of records and arrays.
+
+Author: Ramon Fernandez I Mir and Arthur Charguéraud.
+
+License: MIT.
+
+*)
+
+Set Implicit Arguments.
+Require Export Semantics LibSet LibMap LibList TLCbuffer Typing.
+
+Open Scope Z_scope.
+
+(* ********************************************************************** *)
+(* * Definition of the transformation *)
+
+(** SoA transformation. Specified by:
+    - The typvar of the array of structs.
+    - The typvar of said struct.
+    - The size of the array. *)
+
+Record soa_tr := make_soa_tr {
+  soa_tr_array_name : typvar;
+  soa_tr_struct_name : typvar;
+  soa_tr_struct_fields : set field;
+  soa_tr_array_size : size
+}.
+
+Notation make_soa_tr' := make_soa_tr.
+
+(** Checking if the transformation is acceptable *)
+
+Inductive soa_tr_ok : soa_tr -> typdefctx -> Prop :=
+  | soa_tr_ok_intros : forall Ta Ts fs K Tfs st C,
+      st = make_soa_tr Ta Ts fs K ->
+      Ta \indom C ->
+      Ts \indom C ->
+      C[Ta] = typ_array (typ_var Ts) (Some K) ->
+      C[Ts] = typ_struct Tfs ->
+      fs = dom Tfs ->
+      K > 0%Z ->
+      (forall Tv,
+        Tv \indom C ->
+        Tv <> Ta ->
+        ~ free_typvar C Ta C[Tv]) ->
+      (forall Tv,
+        Tv \indom C ->
+        Tv <> Ts ->
+        ~ free_typvar C Ts C[Tv]) ->
+      soa_tr_ok st C.
+
+
+(* ********************************************************************** *)
+(* * The transformation applied to the different constructs. *)
+
+(** Transformation of typdefctxs: C ~ |C| *)
+
+Inductive tr_typdefctx (st:soa_tr) : typdefctx -> typdefctx -> Prop :=
+  | tr_typdefctx_intro : forall Ta Ts fs K Tfs Tfs' C C',
+      st = make_soa_tr Ta Ts fs K ->
+      dom C' \u \{Ta} = dom C ->
+      Ta \notindom C' ->
+      C[Ta] = typ_array (typ_var Ts) (Some K) ->
+      C[Ts] = typ_struct Tfs ->
+      C'[Ts] = typ_struct Tfs' ->
+      fs = dom Tfs ->
+      dom Tfs = dom Tfs' ->
+      (forall f,
+        f \indom Tfs ->
+        Tfs'[f] = typ_array Tfs[f] (Some K)) ->
+      (forall Tv,
+        Tv \indom C ->
+        Tv <> Ta ->
+        C'[Tv] = C[Tv]) ->
+      tr_typdefctx st C C'.
+
+(** Transformation of paths: π ~ |π| *)
+
+Inductive tr_accesses (st:soa_tr) : accesses -> accesses -> Prop :=
+  | tr_accesses_nil :
+      tr_accesses st nil nil
+  | tr_accesses_soa : forall Ta Ts fs K f T i a0 a1 π a0' a1' π',
+      tr_accesses st π π' ->
+      st = make_soa_tr Ta Ts fs K ->
+      a0 = access_array (typ_var Ts) i ->
+      a1 = access_field T f ->
+      a0' = access_field (typ_array T (Some K)) f ->
+      a1' = access_array T i ->
+      tr_accesses st (a0::a1::π) (a0'::a1'::π')
+  | tr_accesses_array_other : forall π π' T i,
+      T <> typ_var (soa_tr_array_name st) ->
+      tr_accesses st π π' ->
+      tr_accesses st ((access_array T i)::π) ((access_array T i)::π')
+  | tr_accesses_field : forall T π π' f,
+      tr_accesses st π π' ->
+      tr_accesses st ((access_field T f)::π) ((access_field T f)::π').
+
+(** Transformation of values: v ~ |v| *)
+
+Inductive tr_val (st:soa_tr) : val -> val -> Prop :=
+  | tr_val_uninitialized :
+      tr_val st val_uninitialized val_uninitialized
+  | tr_val_unit :
+      tr_val st val_unit val_unit
+  | tr_val_bool : forall b,
+      tr_val st (val_bool b) (val_bool b)
+  | tr_val_int : forall i,
+      tr_val st (val_int i) (val_int i)
+  | tr_val_double : forall d,
+      tr_val st (val_double d) (val_double d)
+  | tr_val_abstract_ptr : forall l π π',
+      tr_accesses st π π' ->
+      tr_val st (val_abstract_ptr l π) (val_abstract_ptr l π')
+  | tr_val_array_tiling : forall fs K Ta a Ts s',
+      st = make_soa_tr Ta Ts fs K ->
+      (forall f a' T,
+        f \in fs ->
+            s'[f] = val_array (typ_array T (Some K)) a'
+        /\  (forall s i,
+              index a' i ->
+                  a[i] = val_struct (typ_var Ts) s
+              /\  tr_val st s[f] a'[i])) ->
+      tr_val st (val_array (typ_var Ta) a) (val_struct (typ_var Ts) s')
+  | tr_val_array_other : forall T a a',
+      T <> typ_var (soa_tr_array_name st) ->
+      length a = length a' ->
+      (forall i,
+        index a i ->
+        tr_val st a[i] a'[i]) ->
+      tr_val st (val_array T a) (val_array T a')
+  | tr_val_struct : forall T s s',
+      dom s = dom s' ->
+      (forall f,
+        f \indom s ->
+        tr_val st s[f] s'[f]) ->
+      tr_val st (val_struct T s) (val_struct T s').
+
+(* Transformation used in the struct cases to avoid repetition. *)
+
+(* let t = t1 in
+   let i = t2 in
+   let j = i / K in
+   let k = i % K in
+     t[j][k] *)
+Inductive tr_prim (tt:tiling_tr) (pr:typ->prim) : trm -> trm -> trm -> Prop :=
+  | tr_access_intro : forall op1 Ta op2 Tt ta1 ta2 K tlk tlj v1 v2,
+      tt = make_tiling_tr Ta Tt K ->
+      op1 = pr (typ_var Ta) ->
+      op2 = pr (typ_var Tt) ->
+      tlk = trm_app binop_mod ((trm_val v2)::(trm_val (val_int K))::nil) ->
+      tlj = trm_app binop_div ((trm_val v2)::(trm_val (val_int K))::nil) ->
+      ta1 = trm_app op1 ((trm_val v1)::tlj::nil) ->
+      ta2 = trm_app op2 (ta1::tlk::nil) ->
+      tr_prim tt pr (trm_val v1) (trm_val v2) ta2.
+
+(* v1[v2 / K][v2 % K] *)
+
+Inductive tr_array_op (tt:tiling_tr) : trm -> trm -> Prop :=
+  | tr_array_op_tiling : forall pr t1 t2 tlt,
+      pr = prim_array_access \/ pr = prim_array_get ->
+      tr_prim tt pr t1 t2 tlt ->
+      tr_array_op tt (trm_app (pr (typ_var (tiling_tr_array_name tt))) (t1::t2::nil)) tlt
+  | tr_array_op_other : forall Ta pr T ts,
+      pr = prim_array_access \/ pr = prim_array_get ->
+      Ta = tiling_tr_array_name tt ->
+      T <> (typ_var Ta) ->
+      tr_array_op tt (trm_app (pr T) ts) (trm_app (pr T) ts).
+
+(** Transformation of terms: t ~ |t| *)
+
+Inductive tr_trm (tt:tiling_tr) : trm -> trm -> Prop :=
+  | tr_trm_val : forall v v',
+      tr_val tt v v' ->
+      tr_trm tt (trm_val v) (trm_val v')
+  | tr_trm_var : forall x,
+      tr_trm tt (trm_var x) (trm_var x)
+  | tr_trm_if : forall t1 t2 t3 t1' t2' t3',
+      tr_trm tt t1 t1' ->
+      tr_trm tt t2 t2' ->
+      tr_trm tt t3 t3' ->
+      tr_trm tt (trm_if t1 t2 t3) (trm_if t1' t2' t3')
+  | tr_trm_let : forall x t1 t2 t1' t2',
+      tr_trm tt t1 t1' ->
+      tr_trm tt t2 t2' ->
+      tr_trm tt (trm_let x t1 t2) (trm_let x t1' t2')
+  (* new *)
+  | tr_trm_new : forall T,
+      tr_trm tt (trm_app (prim_new T) nil) (trm_app (prim_new T) nil)
+  (* Special case: array access *)
+  | tr_trm_array : forall t1' t2' op t1 t2 tr,
+      is_array_op op ->
+      tr_trm tt t1 t1' ->
+      tr_trm tt t2 t2' ->
+      tr_array_op tt (trm_app op (t1'::t2'::nil)) tr ->
+      tr_trm tt (trm_app op (t1::t2::nil)) tr
+  (* Args *)
+  | tr_trm_args1 : forall op t1 t1',
+      tr_trm tt t1 t1' ->
+      tr_trm tt (trm_app op (t1::nil)) (trm_app op (t1'::nil))
+  | tr_trm_args2 : forall op t1 t1' t2 t2',
+      ~ is_array_op op ->
+      tr_trm tt t1 t1' ->
+      tr_trm tt t2 t2' ->
+      tr_trm tt (trm_app op (t1::t2::nil)) (trm_app op (t1'::t2'::nil)).
+
+(** Transformation of stacks: S ~ |S| *)
+
+Inductive tr_stack_item (tt:tiling_tr) : (var * val) -> (var * val) -> Prop :=
+  | tr_stack_item_intro : forall x v v',
+      tr_val tt v v' -> 
+      tr_stack_item tt (x, v) (x, v').
+
+Inductive tr_stack (tt:tiling_tr) : stack -> stack -> Prop :=
+  | tr_stack_intro : forall S S',
+      LibList.Forall2 (tr_stack_item tt) S S' ->
+      tr_stack tt S S'.
+
+(** Transformation of states: m ~ |m| *)
+
+Inductive tr_state (tt:tiling_tr) : state -> state -> Prop :=
+  | tr_state_intro : forall m m',
+      dom m = dom m' ->
+      (forall l,
+        l \indom m ->
+        tr_val tt m[l] m'[l]) ->
+      tr_state tt m m'.
